\documentclass{article}
\usepackage{amsmath}
\begin{document}

\section*{Equations Set 1}
\begin{align*}
x &= \frac{-b \pm \sqrt{b^2 - 4ac}}{2a} \\
  &= \frac{-2 \pm \sqrt{2^2 - 4 \cdot 1 \cdot (-8)}}{2 \cdot 1} \\
  &= \frac{-2 \pm \sqrt{4 + 32}}{2}
\end{align*}

\section*{Equations Set 2}
\begin{align*}
\varphi_{\sigma}^{\lambda} \cdot A_{t} &= \sum_{\pi \in C_{t}} \text{sgn}(\pi) \varphi_{\sigma}^{\lambda} \varphi_{\pi}^{\lambda} \\
&= \sum_{\tau \in C_{\sigma}^{t}} \text{sgn}(\sigma^{-1} \tau \sigma) \varphi_{\sigma}^{\lambda} \varphi_{\sigma^{-1} \tau \sigma}^{\lambda} \\
&= A_{\sigma}^{t} \varphi_{\sigma}^{\lambda}
\end{align*}

\end{document}
